Matroid/Connectivity/Fan/Minor.lean
@@ -22,34 +22,33 @@ namespace Matroid
 spanned by the contract-set. -/
 lemma IsFan.contract (hF : M.IsFan F b c) (X : Set α) (hX : _root_.Disjoint {e | e ∈ F} X)
     (h0 : b = false → F[0] ∉ M.closure X) (hlast : c = false → F[F.length - 1] ∉ M.closure X)
-    (h2 : F.length = 2 → F[(!b).toNat] ∉ M.closure X := by lia)
     (h3 : F.length = 3 → b = false → c = false → M.Skew {e | e ∈ F} (X ∩ M.E) := by lia) :
     (M ／ X).IsFan F b c := by
-  refine isFan_of_eq_of_forall_triangle hF.two_le_length hF.nodup (by simp [hF.length_bodd_eq])
+  have hFX : ∀ {i} {hi : i < F.length}, F[i] ∉ X := by grind
+  refine isFan_of_eq_of_forall_isCircuit hF.two_le_length hF.nodup (by simp [hF.length_bodd_eq])
     ?_ fun i hi ↦ ?_
-  · rintro hF2 (rfl | rfl) i hi
+  · rintro hF2 i hi
     · obtain rfl | rfl := b
       · obtain rfl | rfl : i = 0 ∨ i = 1 := by grind
         · simp [h0, hF.getElem_mem_ground]
-        simpa [hF.getElem_mem_ground] using h2 hF2
+        simpa [hFX] using hF.dual.isNonloop_getElem 1 hi (by simp)
       obtain rfl | rfl : i = 0 ∨ i = 1 := by grind
-      · simpa [hF.getElem_mem_ground] using h2 hF2
+      · simpa [hFX] using hF.dual.isNonloop_getElem 0 hi (by simp)
       have h1cl : F[1] ∉ M.closure X := by simpa [hF.bool_right_eq, hF2] using hlast
       simpa [hF.getElem_mem_ground]
-    simpa [hX.notMem_of_mem_left] using hF.isNonloop_bDual (e := F[i]) (by simp) true
   obtain rfl | hb := b.eq_or_eq_not !i.bodd
-  · simpa [hX.notMem_of_mem_left] using hF.isTriangle_getElem i (by lia)
+  · simpa [hFX] using (hF.isTriangle_getElem i (by lia)).isCircuit
   suffices hsk : M.Skew {F[i], F[i + 1], F[i + 2]} (X ∩ M.E) by
-    simpa [hb] using (hF.isTriangle_getElem_of_eq i (by simp [hb])).contract_isTriangle
-      hsk.symm
-  clear h2
+    simpa [hb] using ((hF.isTriangle_getElem_of_eq i (by simp [hb])).contract_isTriangle
+      hsk.symm).isCircuit
+  -- clear hX
   wlog h1 : i + 3 ≠ F.length generalizing i F b c with aux
   · replace h1 : i + 3 = F.length := by simpa using h1
     obtain rfl | i := i
     · exact (h3 (by simp [← h1]) (by simp [hb])
         (by simp [hF.bool_right_eq, hb, ← h1])).mono_left <| by simp [insert_subset_iff]
-    specialize aux hF.reverse (by simpa) (by simpa) (by simpa)
-      (fun h hc hb ↦ by simpa using h3 (by simpa using h) hb hc) 0 (by grind)
+    specialize aux hF.reverse (by simpa) (by simpa) (by grind)
+      (fun h hc hb ↦ by simpa using h3 (by simpa using h) hb hc) (by grind) 0 (by grind)
       (by simp [hF.bool_right_eq, hb, ← h1]) (by grind)
     rw [pair_comm, insert_comm, pair_comm]
     cases b with simpa [hF.bool_right_eq, ← h1] using aux
@@ -74,30 +73,94 @@ lemma IsFan.contract (hF : M.IsFan F b c) (X : Set α) (hX : _root_.Disjoint {e 
   rw [(hF.isTriad_getElem_of_eq i (by simp [hb])).reverse.mem_iff_mem_of_isCircuit hC hi1] at hiC
   simpa [hX.notMem_of_mem_left, hF.nodup.getElem_inj_iff, add_assoc] using hCss hiC
 
+/-- If `N` is a minor of `M`, and `F` is a fan of `M` contained in `E(N)`, whose (co)joint ends are
+are not (co)loops of `N`, then `F` is also a fan of `N`.  -/
+lemma IsFan.minor {N : Matroid α} (hF : M.IsFan F b c) (h4 : 4 ≤ F.length) (hNM : N ≤m M)
+    (hFN : {e | e ∈ F} ⊆ N.E) (h_first : (N.bDual b).IsNonloop F[0])
+    (h_last : (N.bDual c).IsNonloop F[F.length - 1]) : N.IsFan F b c := by
+  obtain ⟨C, D, hC, hD, hCD, rfl⟩ := hNM.exists_eq_contract_delete_disjoint
+  have hCF := hF.contract (X := C) (by grind) ?_ ?_
+  · have hwin := (hCF.dual.contract (X := D) (by grind) ?_ ?_).dual
+    · simpa using hwin
+    · simp only [Bool.not_eq_eq_eq_not, Bool.not_false, dual_contract, delete_closure_eq, mem_sdiff,
+        not_and, not_not, hCD.sdiff_eq_right]
+      rintro rfl hcl
+      refine False.elim <| h_first.not_isLoop ?_
+      grind [bDual_true, dual_delete, dual_contract, contract_isLoop_iff_mem_closure,
+        delete_closure_eq, hCD.sdiff_eq_right]
+    simp only [Bool.not_eq_eq_eq_not, Bool.not_false, dual_contract, delete_closure_eq, mem_sdiff]
+    rintro rfl hcl
+    refine h_last.not_isLoop ?_
+    grind [bDual_true, dual_delete, dual_contract, contract_isLoop_iff_mem_closure,
+      delete_closure_eq]
+  · rintro rfl hcl
+    grind [bDual_false, delete_isLoop_iff, contract_isLoop_iff_mem_closure, h_first.not_isLoop]
+  rintro rfl hcl
+  grind [h_last.not_isLoop, bDual_false, delete_isLoop_iff, contract_isLoop_iff_mem_closure]
+
+lemma isFan_delete_iff_of_subset_loops {X : Set α} (hX : X ⊆ M.loops)
+    (hFX : _root_.Disjoint X {e | e ∈ F}) : (M ＼ X).IsFan F b c ↔ M.IsFan F b c := by
+  have hrw (C : Set α) (d : Bool) (hCX : Disjoint X C) :
+      ((M ＼ X).bDual d).IsCircuit C ↔ (M.bDual d).IsCircuit C := by
+    cases d
+    · simp [hCX.symm]
+    simp only [bDual_true, dual_delete]
+    rw [contract_eq_delete_of_subset_coloops (by simpa), delete_isCircuit_iff,
+      and_iff_left hCX.symm]
+  simp only [isFan_iff_forall']
+  convert Iff.rfl using 7 with a i i
+  · convert Iff.rfl using 2 with hi
+    rw [isNonloop_iff, ← singleton_isCircuit, hrw _ _ (by grind), bDual_ground, delete_ground,
+      mem_sdiff, isNonloop_iff, ← singleton_isCircuit, bDual_ground,
+      and_iff_left (show F[i] ∉ X by grind)]
+  rw [hrw _ _ (hFX.mono_right (by grind))]
+
+/- Restrict usually preserve the property of being a fan -/
+lemma IsFan.restrict (hF : M.IsFan F b c) (X : Set α) (hX : {e | e ∈ F} ⊆ X)
+    (h0 : b = true → F[0] ∈ M.closure (X \ {F[0]}))
+    (hlast : c = true → F[F.length - 1] ∈ M.closure (X \ {F[F.length - 1]}))
+    (h3 : F.length = 3 → b = true → c = true → M✶.Skew {e | e ∈ F} (M.E \ X) := by lia) :
+    (M ↾ X).IsFan F b c := by
+  wlog hXE : X ⊆ M.E generalizing X with aux
+  · specialize aux (X ∩ M.E) (subset_inter hX hF.subset_ground)
+    rw [inter_sdiff_right_comm, inter_sdiff_right_comm, closure_inter_ground, closure_inter_ground,
+      imp_iff_right h0, imp_iff_right hlast, sdiff_inter_self_eq_sdiff, imp_iff_right h3,
+      imp_iff_right inter_subset_right] at aux
+    rwa [← isFan_delete_iff_of_subset_loops (X := X \ M.E), delete_eq_restrict, restrict_ground_eq,
+      restrict_restrict_eq _ sdiff_subset, sdiff_sdiff_right_self]
+    · grw [restrict_loops_eq', ← subset_union_right]
+    grw [hF.subset_ground]
+    exact disjoint_sdiff_left
+  rw [← delete_compl, ← b.not_not, ← c.not_not, ← isFan_dual_iff, dual_delete]
+  refine hF.dual.contract _ (disjoint_sdiff_right.mono_left hX) ?_ ?_ ?_
+  · rwa [Bool.not_eq_eq_eq_not, Bool.not_false,
+      mem_dual_closure_iff_notMem_closure_compl, sdiff_sdiff_cancel_left hXE, not_not]
+    simp [show F[0] ∈ X from hX (by simp)]
+  · rwa [Bool.not_eq_eq_eq_not, Bool.not_false,
+      mem_dual_closure_iff_notMem_closure_compl, sdiff_sdiff_cancel_left hXE, not_not]
+    simp [show F[F.length - 1] ∈ X from hX (by simp)]
+  simpa [inter_eq_self_of_subset_left sdiff_subset]
+
+/-- Contracting the head of a fan usually gives a fan on the tail. -/
 lemma IsFan.contract_head (hF : M.IsFan F b c) (hF3 : 3 ≤ F.length)
     (h_init : b = true → ¬ M.Parallel F[0] F[1])
     (h_false : b = false → c = false → ¬ M.Parallel F[0] F[F.length - 1])
-    (h4 : ∀ (hF : F.length = 4), b = true → ¬ F[0] ∈ M.closure {F[1], F[2]} := by lia)
-    (h3 : ∀ (hF : F.length = 3), b = true → ¬ M.Parallel F[0] F[2] := by lia) :
+    (h4 : F.length = 4 → b = true → ¬ F[0] ∈ M.closure {F[1], F[2]} := by lia) :
     (M ／ {F[0]}).IsFan F.tail (!b) c := by
   have aux := @IsFan.contract _ M F.tail _ _ (hF.tail hF3) {F[0]}
     (by simp [getElem_zero_eq_head, hF.nodup.head_notMem_tail])
   simp only [Bool.not_eq_eq_eq_not, Bool.not_false, getElem_tail, zero_add, getElem_mem,
     ← IsNonloop.parallel_iff_mem_closure (hF.isNonloop _), parallel_comm (f := F[0]), length_tail,
     show F.length - 1 - 1 + 1 = F.length - 1 by lia, Nat.pred_eq_succ_iff, Nat.reduceAdd,
-    Bool.not_not, singleton_inter_of_mem hF.getElem_mem_ground] at aux
-  refine aux h_init ?_ ?_ ?_
+    imp_iff_right h_init, singleton_inter_of_mem hF.getElem_mem_ground] at aux
+  refine aux ?_ ?_
   · rintro rfl hpara
     obtain rfl | rfl := b
     · exact h_false rfl rfl hpara
     have hwin := (hF.isTriangle_getElem 0 (by lia)).isCircuit.mem_iff_mem_of_parallel_bDual hpara
     obtain h3' : F.length = 3 := by simpa
       [hF.nodup.getElem_inj_iff, show F.length - 1 ≠ 0 by lia, show F.length ≠ 2 by lia] using hwin
-    exact h3 h3' rfl <| by simpa [h3'] using hpara
-  · obtain rfl | rfl := b
-    · exact fun h3 hpara ↦ by simpa [hF.nodup.getElem_inj_iff] using
-        (hF.isTriangle_getElem 0 (by lia)).notMem_of_mem_of_parallel hpara
-    simpa using h3
+    simpa [h3'] using hF.length_bodd_eq
   rintro hF4 rfl rfl
   rw! [(hF.isNonloop (by simp)).skew_right_iff (hF.tail hF3).subset_ground,
     (eq_of_length_eq_three (l := F.tail)) (by grind), getElem_tail, getElem_tail, getElem_tail]
@@ -106,16 +169,18 @@ lemma IsFan.contract_head (hF : M.IsFan F b c) (hF3 : 3 ≤ F.length)
   rw [pair_comm, closure_insert_eq_of_mem_closure]
   exact (hF.isTriangle_getElem_of_eq 1 rfl).mem_closure₃
 
-lemma IsFan.delete_head (hF : M.IsFan F b c) (h5 : 5 ≤ F.length)
+lemma IsFan.delete_head (hF : M.IsFan F b c) (h3 : 3 ≤ F.length)
     (h_init : b = false → ¬ M✶.Parallel F[0] F[1])
-    (h_pair : b = true → c = true → ¬ M✶.Parallel F[0] F[F.length - 1]) :
+    (h_pair : b = true → c = true → ¬ M✶.Parallel F[0] F[F.length - 1])
+    (h4 : F.length = 4 → b = false → ¬ F[0] ∈ M✶.closure {F[1], F[2]} := by lia) :
     (M ＼ {F[0]}).IsFan F.tail (!b) c := by
   simpa using (hF.dual.contract_head (by lia) (by simpa) (by simpa)).dual
 
-lemma IsFan.remove_head (hF : M.IsFan F b c) (h5 : 5 ≤ F.length) {d : Bool}
+lemma IsFan.remove_head (hF : M.IsFan F b c) (h3 : 3 ≤ F.length) {d : Bool}
     (h_init : b = d → ¬ (M.bDual !d).Parallel F[0] F[1])
-    (h_pair : b = !d → c = !d → ¬ (M.bDual !d).Parallel F[0] F[F.length - 1]) :
+    (h_pair : b = !d → c = !d → ¬ (M.bDual !d).Parallel F[0] F[F.length - 1])
+    (h4 : F.length = 4 → b = d → ¬ F[0] ∈ (M.bDual !d).closure {F[1], F[2]} := by lia):
     (M.remove d {F[0]}).IsFan F.tail (!b) c := by
   obtain rfl | rfl := d
-  · exact hF.delete_head h5 (by simpa) (by simpa)
-  exact hF.contract_head (by lia) (by simpa) (by simpa)
+  · exact hF.delete_head h3 (by simpa) (by simpa) (by simpa using h4)
+  exact hF.contract_head h3 (by simpa) (by simpa) (by simpa using h4)
